SoftwareFoundations/ProgrammingLanguageFoundations.lean
@@ -5,3 +5,4 @@ import «SoftwareFoundations».«ProgrammingLanguageFoundations».«HoareAsLogic
 import «SoftwareFoundations».«ProgrammingLanguageFoundations».«SmallStep»
 import «SoftwareFoundations».«ProgrammingLanguageFoundations».«Types»
 import «SoftwareFoundations».«ProgrammingLanguageFoundations».«Stlc»
+import «SoftwareFoundations».«ProgrammingLanguageFoundations».«StlcProp»
